generational/spec/GC.Gen.MinorCollectForwarding.NormalEdges.fsti
@@ -87,7 +87,7 @@ val combined_reachable_edge_forwarded_normal
       RBridge.roots_valid_nonblue roots major /\
       CheneyBFS.cheney_no_oom minor major fp roots /\
       (let cg = CG.build_combined_graph minor major in
-       let combined_roots = CG.classify_roots roots in
+       let combined_roots = CG.classify_roots minor roots in
        CG.combined_reachable cg combined_roots u /\
        CG.combined_reachable cg combined_roots v /\
        CG.mem_ce (u, v) cg) /\
@@ -102,7 +102,7 @@ val combined_reachable_edge_forwarded_normal
 let fwd_disjoint_reachable_major
   (minor: minor_state) (major: heap) (fp: U64.t) (roots: seq U64.t) : prop =
   let cg = CG.build_combined_graph minor major in
-  let combined_roots = CG.classify_roots roots in
+  let combined_roots = CG.classify_roots minor roots in
   let prom = cheney_promote minor major fp roots in
   forall (x y: U64.t).
     CG.combined_reachable cg combined_roots (CG.MinorV x) /\
@@ -146,14 +146,14 @@ let normal_src_reachable
   (minor: minor_state) (major: heap) (fp: U64.t) (roots: seq U64.t)
   (u: CG.combined_vertex) : prop =
   let cg = CG.build_combined_graph minor major in
-  let combined_roots = CG.classify_roots roots in
+  let combined_roots = CG.classify_roots minor roots in
   CG.combined_reachable cg combined_roots u /\
   normal_vertex_ready minor major fp roots u
 
 let combined_reachable_normal_injective_prop
   (minor: minor_state) (major: heap) (fp: U64.t) (roots: seq U64.t) : prop =
   let cg = CG.build_combined_graph minor major in
-  let combined_roots = CG.classify_roots roots in
+  let combined_roots = CG.classify_roots minor roots in
   let prom = cheney_promote minor major fp roots in
   forall (u v: CG.combined_vertex).
     CG.combined_reachable cg combined_roots u /\
